theories/Operational/Awkernel/Minimal/WorkloadAcceptanceExtraction.v
@@ -11,4 +11,6 @@ Extraction "/scheduling_theory/extracted/haskell/AwkernelWorkloadAcceptance.hs"
   AwkernelSchedTraceEntry
   awk_workload_accepts_sched_trace
   first_non_fifo_sched_trace_index
-  awk_workload_accepts_global_fifo_sched_trace.
+  first_non_scheduler_relation_sched_trace_index
+  awk_workload_accepts_global_fifo_sched_trace
+  awk_workload_accepts_global_fifo_scheduler_relation_sched_trace.
